Add intended theorems to prove

isabelle/Auction.thy
@@ -1,5 +1,5 @@
 theory Auction
-imports Semantics ValidState
+imports Semantics ValidState CloseSafe
 begin
 
 definition bid :: ByteString where
@@ -59,6 +59,14 @@ where
 
   by pat_completeness auto
 
-fun contract :: "Party \<Rightarrow> int \<Rightarrow> int \<Rightarrow> Party list \<Rightarrow> Slot \<Rightarrow> Contract" where
-"contract own mBid MBid bidders ddl = (contractLoop None [] bidders \<lparr>owner = own, minBid = mBid, maxBid = MBid, deadline = ddl\<rparr>)" 
+fun auction :: "Party \<Rightarrow> int \<Rightarrow> int \<Rightarrow> Party list \<Rightarrow> Slot \<Rightarrow> Contract" where
+"auction own mBid MBid bidders ddl = (contractLoop None [] bidders \<lparr>owner = own, minBid = mBid, maxBid = MBid, deadline = ddl\<rparr>)" 
 
+
+lemma auctionComputeTransactionIsSafe : "computeTransaction tra sta (auction own mBid MBid bidders ddl)  = TransactionOutput trec \<Longrightarrow> 
+                         txOutWarnings trec = []"
+  oops
+
+theorem auctionPlayTraceIsSafe : "playTrace sl (auction own mBid MBid bidders ddl) t = TransactionOutput trec \<Longrightarrow>
+                                  txOutWarnings trec = []"
+  oops
